Weidenbach_Book/IsaSAT_Setup.thy
@@ -300,21 +300,6 @@ definition isasat_fast_slow :: \<open>twl_st_wl_heur \<Rightarrow> twl_st_wl_heu
       RETURN (trail_fast_of_slow M', N', D', Q', convert_wlists_to_nat_conv W', vm, \<phi>,
         clvls, cach, lbd, outl, stats))\<close>
 
-sepref_thm isasat_fast_slow_code
-  is \<open>isasat_fast_slow\<close>
-  :: \<open>isasat_fast_assn\<^sup>d \<rightarrow>\<^sub>a isasat_assn\<close>
-  unfolding isasat_fast_assn_def isasat_assn_def isasat_fast_slow_def
-  by sepref
-
-concrete_definition (in -) isasat_fast_slow_code
-  uses isasat_input_ops.isasat_fast_slow_code.refine_raw
-  is \<open>(?f, _) \<in> _\<close>
-
-prepare_code_thms (in -) isasat_fast_slow_code_def
-
-lemmas isasat_fast_slow_code[sepref_fr_rules] =
-   isasat_fast_slow_code.refine
-
 type_synonym (in -) twl_st_wl_heur_W_list =
   \<open>(nat,nat) ann_lits \<times> nat clauses_l \<times>
     nat cconflict \<times> nat clause_l \<times> nat list list \<times> vmtf_remove_int \<times> bool list \<times> nat \<times>
